src/tactics/FStar.Tactics.V2.Primops.fst
@@ -275,4 +275,7 @@ let ops = [
     #_ #(TI.e_tactic_thunk e_unit) #_ #_ #_
     #_ #(TI.e_tactic_nbe_thunk NBET.e_unit) #_ #_ #_
     call_subtac call_subtac;
+
+  mk_tac_step_4 0 "call_subtac_tm"
+    call_subtac_tm call_subtac_tm;
 ]
